Semantic/CoreCapybara/Denotation/KripkeModel.lean
@@ -190,6 +190,7 @@ theorem kdenot_mono (T : Ty .capt {}) {k : Nat} {st1 st2 m1 m2} (hw : WorldLe st
   | .cap _ => by unfold kdenot at ht ⊢; exact ht
   | .poly _ _ _ => by unfold kdenot at ht ⊢; exact ht
   | .cpoly _ _ _ => by unfold kdenot at ht ⊢; exact ht
+  | .consumer _ _ _ => by unfold kdenot at ht ⊢; exact ht
   | .modal _ _ _ => by unfold kdenot at ht ⊢; exact ht
 termination_by sizeOf T
 decreasing_by all_goals (simp_wf; try omega)
@@ -219,6 +220,7 @@ theorem kdenot_down (st : StoreTyping) (T : Ty .capt {}) {k : Nat} (m : Memory)
   | .bool => by unfold kdenot at ht ⊢; exact ht
   | .poly _ _ _ => by unfold kdenot at ht ⊢; exact ht
   | .cpoly _ _ _ => by unfold kdenot at ht ⊢; exact ht
+  | .consumer _ _ _ => by unfold kdenot at ht ⊢; exact ht
   | .modal _ _ _ => by unfold kdenot at ht ⊢; exact ht
 termination_by sizeOf T
 decreasing_by all_goals (simp_wf; try omega)
